<rdf:RDF
    xmlns:rdf="http://www.w3.org/1999/02/22-rdf-syntax-ns#"
    xmlns:foaf="http://xmlns.com/foaf/0.1/"
    xmlns:d2r="http://sites.wiwiss.fu-berlin.de/suhl/bizer/d2r-server/config.rdf#"
    xmlns:owl="http://www.w3.org/2002/07/owl#"
    xmlns:dc="http://purl.org/dc/elements/1.1/"
    xmlns:xsd="http://www.w3.org/2001/XMLSchema#"
    xmlns:rdfs="http://www.w3.org/2000/01/rdf-schema#"
    xmlns:d2rq="http://www.wiwiss.fu-berlin.de/suhl/bizer/D2RQ/0.1#">
  <owl:Ontology rdf:about="">
    <dc:creator rdf:resource="http://richard.cyganiak.de/foaf.rdf#cygri"/>
    <foaf:page>
      <rdf:Description rdf:about="http://sites.wiwiss.fu-berlin.de/suhl/bizer/d2r-server/">
        <rdfs:label xml:lang="en">D2R Server homepage and documentation</rdfs:label>
      </rdf:Description>
    </foaf:page>
    <rdfs:comment xml:lang="en">This vocabulary defines RDF terms used in configuration files for D2R Server, a software application that publishes relational databases on the Semantic Web.</rdfs:comment>
    <rdfs:label xml:lang="en">D2R Server configuration vocabulary</rdfs:label>
  </owl:Ontology>
  <rdfs:Class rdf:about="http://sites.wiwiss.fu-berlin.de/suhl/bizer/d2r-server/config.rdf#Server">
    <rdfs:isDefinedBy rdf:resource=""/>
    <rdfs:comment xml:lang="en">A configuration for a D2R Server installation.</rdfs:comment>
    <rdfs:label xml:lang="en">Server</rdfs:label>
  </rdfs:Class>
  <rdf:Property rdf:about="http://sites.wiwiss.fu-berlin.de/suhl/bizer/d2r-server/config.rdf#metadataTemplate">
    <rdfs:isDefinedBy rdf:resource=""/>
    <rdfs:domain rdf:resource="http://sites.wiwiss.fu-berlin.de/suhl/bizer/d2r-server/config.rdf#Server"/>
    <rdfs:comment xml:lang="en">A RDF metadata template.</rdfs:comment>
    <rdfs:label xml:lang="en">metadata template</rdfs:label>
  </rdf:Property>
  <rdf:Property rdf:about="http://sites.wiwiss.fu-berlin.de/suhl/bizer/d2r-server/config.rdf#pageTimeout">
    <rdfs:isDefinedBy rdf:resource=""/>
    <rdfs:range rdf:resource="http://www.w3.org/2001/XMLSchema#decimal"/>
    <rdfs:domain rdf:resource="http://sites.wiwiss.fu-berlin.de/suhl/bizer/d2r-server/config.rdf#Server"/>
    <rdfs:comment xml:lang="en">Timeout for generating HTML pages and RDF descriptions, in seconds. 0 for no timeout.</rdfs:comment>
    <rdfs:label>Page timeout</rdfs:label>
  </rdf:Property>
  <rdf:Property rdf:about="http://sites.wiwiss.fu-berlin.de/suhl/bizer/d2r-server/config.rdf#datasetMetadataTemplate">
    <rdfs:isDefinedBy rdf:resource=""/>
    <rdfs:domain rdf:resource="http://sites.wiwiss.fu-berlin.de/suhl/bizer/d2r-server/config.rdf#Server"/>
    <rdfs:comment xml:lang="en">A RDF dataset metadata template.</rdfs:comment>
    <rdfs:label xml:lang="en">dataset metadata template</rdfs:label>
  </rdf:Property>
  <rdf:Property rdf:about="http://sites.wiwiss.fu-berlin.de/suhl/bizer/d2r-server/config.rdf#publishes">
    <rdfs:isDefinedBy rdf:resource=""/>
    <rdfs:range rdf:resource="http://www.wiwiss.fu-berlin.de/suhl/bizer/D2RQ/0.1#Database"/>
    <rdfs:domain rdf:resource="http://sites.wiwiss.fu-berlin.de/suhl/bizer/d2r-server/config.rdf#Server"/>
    <rdfs:comment xml:lang="en">The D2RQ-mapped database that is published by a D2R Server installation.</rdfs:comment>
    <rdfs:label xml:lang="en">publishes</rdfs:label>
  </rdf:Property>
  <rdf:Property rdf:about="http://sites.wiwiss.fu-berlin.de/suhl/bizer/d2r-server/config.rdf#limitPerPropertyBridge">
    <rdfs:isDefinedBy rdf:resource=""/>
    <rdfs:range rdf:resource="http://www.w3.org/2000/01/rdf-schema#Literal"/>
    <rdfs:domain rdf:resource="http://sites.wiwiss.fu-berlin.de/suhl/bizer/d2r-server/config.rdf#Server"/>
    <rdfs:comment xml:lang="en">Maximum number of values for each property bridge that will be displayed in the web interface when browsing resources. A value of false means no limit.</rdfs:comment>
    <rdfs:label xml:lang="en">Limit per property bridge</rdfs:label>
  </rdf:Property>
  <rdf:Property rdf:about="http://sites.wiwiss.fu-berlin.de/suhl/bizer/d2r-server/config.rdf#autoReloadMapping">
    <rdfs:isDefinedBy rdf:resource=""/>
    <rdfs:domain rdf:resource="http://sites.wiwiss.fu-berlin.de/suhl/bizer/d2r-server/config.rdf#Server"/>
    <rdfs:comment xml:lang="en">Whether D2R Server should check for an updated mapping file with every request.</rdfs:comment>
    <rdfs:label xml:lang="en">automatically check for updated mapping file</rdfs:label>
  </rdf:Property>
  <rdf:Property rdf:about="http://sites.wiwiss.fu-berlin.de/suhl/bizer/d2r-server/config.rdf#baseURI">
    <rdfs:isDefinedBy rdf:resource=""/>
    <rdfs:domain rdf:resource="http://sites.wiwiss.fu-berlin.de/suhl/bizer/d2r-server/config.rdf#Server"/>
    <rdfs:comment xml:lang="en">Base URI for a D2R Server installation; the URI of the running server's start page.</rdfs:comment>
    <rdfs:label xml:lang="en">server base URI</rdfs:label>
  </rdf:Property>
  <rdf:Property rdf:about="http://sites.wiwiss.fu-berlin.de/suhl/bizer/d2r-server/config.rdf#documentMetadata">
    <rdfs:isDefinedBy rdf:resource=""/>
    <rdfs:domain rdf:resource="http://sites.wiwiss.fu-berlin.de/suhl/bizer/d2r-server/config.rdf#Server"/>
    <rdfs:comment xml:lang="en">A template resource whose properties will be attached as metadata to all RDF documents published by a D2R Server installation.</rdfs:comment>
    <rdfs:label xml:lang="en">document metadata</rdfs:label>
  </rdf:Property>
  <rdf:Property rdf:about="http://sites.wiwiss.fu-berlin.de/suhl/bizer/d2r-server/config.rdf#vocabularyIncludeInstances">
    <rdfs:isDefinedBy rdf:resource=""/>
    <rdfs:domain rdf:resource="http://sites.wiwiss.fu-berlin.de/suhl/bizer/d2r-server/config.rdf#Server"/>
    <rdfs:comment xml:lang="en">Whether views of vocabulary resources should include instance data.</rdfs:comment>
    <rdfs:label xml:lang="en">serve instance data for vocabulary resources</rdfs:label>
  </rdf:Property>
  <rdf:Property rdf:about="http://sites.wiwiss.fu-berlin.de/suhl/bizer/d2r-server/config.rdf#port">
    <rdfs:isDefinedBy rdf:resource=""/>
    <rdfs:domain rdf:resource="http://sites.wiwiss.fu-berlin.de/suhl/bizer/d2r-server/config.rdf#Server"/>
    <rdfs:comment xml:lang="en">The TCP port on which a D2R Server installation listens.</rdfs:comment>
    <rdfs:label xml:lang="en">server port</rdfs:label>
  </rdf:Property>
  <rdf:Property rdf:about="http://sites.wiwiss.fu-berlin.de/suhl/bizer/d2r-server/config.rdf#enableMetadata">
    <rdfs:isDefinedBy rdf:resource=""/>
    <rdfs:domain rdf:resource="http://sites.wiwiss.fu-berlin.de/suhl/bizer/d2r-server/config.rdf#Server"/>
    <rdfs:comment xml:lang="en">Whether to enable all metadata generation.</rdfs:comment>
    <rdfs:label xml:lang="en">enable metadata generation</rdfs:label>
  </rdf:Property>
  <rdf:Property rdf:about="http://sites.wiwiss.fu-berlin.de/suhl/bizer/d2r-server/config.rdf#sparqlTimeout">
    <rdfs:isDefinedBy rdf:resource=""/>
    <rdfs:range rdf:resource="http://www.w3.org/2001/XMLSchema#decimal"/>
    <rdfs:domain rdf:resource="http://sites.wiwiss.fu-berlin.de/suhl/bizer/d2r-server/config.rdf#Server"/>
    <rdfs:comment xml:lang="en">Timeout for executing SPARQL queries, in seconds. 0 for no timeout.</rdfs:comment>
    <rdfs:label>SPARQL timeout</rdfs:label>
  </rdf:Property>
  <rdf:Property rdf:about="http://sites.wiwiss.fu-berlin.de/suhl/bizer/d2r-server/config.rdf#limitPerClassMap">
    <rdfs:isDefinedBy rdf:resource=""/>
    <rdfs:range rdf:resource="http://www.w3.org/2000/01/rdf-schema#Literal"/>
    <rdfs:domain rdf:resource="http://sites.wiwiss.fu-berlin.de/suhl/bizer/d2r-server/config.rdf#Server"/>
    <rdfs:comment xml:lang="en">Maximum number of values for each class map that will be displayed in the web interface when browsing resources. A value of false means no limit.</rdfs:comment>
    <rdfs:label xml:lang="en">Limit per class map</rdfs:label>
  </rdf:Property>
</rdf:RDF>
