@prefix d2r:  <http://sites.wiwiss.fu-berlin.de/suhl/bizer/d2r-server/config.rdf#> .
@prefix rdf:  <http://www.w3.org/1999/02/22-rdf-syntax-ns#> .
@prefix rdfs: <http://www.w3.org/2000/01/rdf-schema#> .
@prefix owl:  <http://www.w3.org/2002/07/owl#> .
@prefix dc:   <http://purl.org/dc/elements/1.1/> .
@prefix foaf: <http://xmlns.com/foaf/0.1/> .
@prefix d2rq: <http://www.wiwiss.fu-berlin.de/suhl/bizer/D2RQ/0.1#> .
@prefix xsd:  <http://www.w3.org/2001/XMLSchema#> .

<> a owl:Ontology;
    rdfs:label "D2R Server configuration vocabulary"@en;
    rdfs:comment "This vocabulary defines RDF terms used in configuration files for D2R Server, a software application that publishes relational databases on the Semantic Web."@en;
    foaf:page <http://sites.wiwiss.fu-berlin.de/suhl/bizer/d2r-server/>;
    dc:creator <http://richard.cyganiak.de/foaf.rdf#cygri>;
    .
<http://sites.wiwiss.fu-berlin.de/suhl/bizer/d2r-server/>
    rdfs:label "D2R Server homepage and documentation"@en;
    .
d2r:Server a rdfs:Class;
    rdfs:label "Server"@en;
    rdfs:comment "A configuration for a D2R Server installation."@en;
    rdfs:isDefinedBy <>;
    .
d2r:baseURI a rdf:Property;
    rdfs:label "server base URI"@en;
    rdfs:comment "Base URI for a D2R Server installation; the URI of the running server's start page."@en;
    rdfs:domain d2r:Server;
    rdfs:isDefinedBy <>;
    .
d2r:port a rdf:Property;
    rdfs:label "server port"@en;
    rdfs:comment "The TCP port on which a D2R Server installation listens."@en;
    rdfs:domain d2r:Server;
    rdfs:isDefinedBy <>;
    .
d2r:publishes a rdf:Property;
    rdfs:label "publishes"@en;
    rdfs:comment "The D2RQ-mapped database that is published by a D2R Server installation."@en;
    rdfs:domain d2r:Server;
    rdfs:range d2rq:Database;
    rdfs:isDefinedBy <>;
    .
d2r:documentMetadata a rdf:Property;
    rdfs:label "document metadata"@en;
    rdfs:comment "A template resource whose properties will be attached as metadata to all RDF documents published by a D2R Server installation."@en;
    rdfs:domain d2r:Server;
    rdfs:isDefinedBy <>;
    .
d2r:vocabularyIncludeInstances a rdf:Property;
    rdfs:label "serve instance data for vocabulary resources"@en;
    rdfs:comment "Whether views of vocabulary resources should include instance data."@en;
    rdfs:domain d2r:Server;
    rdfs:isDefinedBy <>;
    .
d2r:autoReloadMapping a rdf:Property;
    rdfs:label "automatically check for updated mapping file"@en;
    rdfs:comment "Whether D2R Server should check for an updated mapping file with every request."@en;
    rdfs:domain d2r:Server;
    rdfs:isDefinedBy <>;
    .
d2r:metadataTemplate a rdf:Property;
    rdfs:label "metadata template"@en;
    rdfs:comment "A RDF metadata template."@en;
    rdfs:domain d2r:Server;
    rdfs:isDefinedBy <>;
    .
d2r:datasetMetadataTemplate a rdf:Property;
    rdfs:label "dataset metadata template"@en;
    rdfs:comment "A RDF dataset metadata template."@en;
    rdfs:domain d2r:Server;
    rdfs:isDefinedBy <>;
    .
d2r:enableMetadata a rdf:Property;
    rdfs:label "enable metadata generation"@en;
    rdfs:comment "Whether to enable all metadata generation."@en;
    rdfs:domain d2r:Server;
    rdfs:isDefinedBy <>;
    .
d2r:limitPerClassMap a rdf:Property;
    rdfs:label "Limit per class map"@en;
    rdfs:comment "Maximum number of values for each class map that will be displayed in the web interface when browsing resources. A value of false means no limit."@en;
    rdfs:domain d2r:Server;
    rdfs:range rdfs:Literal;
    rdfs:isDefinedBy <>;
    .
d2r:limitPerPropertyBridge a rdf:Property;
    rdfs:label "Limit per property bridge"@en;
    rdfs:comment "Maximum number of values for each property bridge that will be displayed in the web interface when browsing resources. A value of false means no limit."@en;
    rdfs:domain d2r:Server;
    rdfs:range rdfs:Literal;
    rdfs:isDefinedBy <>;
    .
d2r:sparqlTimeout a rdf:Property;
    rdfs:label "SPARQL timeout";
    rdfs:comment "Timeout for executing SPARQL queries, in seconds. 0 for no timeout."@en;
    rdfs:domain d2r:Server;
    rdfs:range xsd:decimal;
    rdfs:isDefinedBy <>;
    .
d2r:pageTimeout a rdf:Property;
    rdfs:label "Page timeout";
    rdfs:comment "Timeout for generating HTML pages and RDF descriptions, in seconds. 0 for no timeout."@en;
    rdfs:domain d2r:Server;
    rdfs:range xsd:decimal;
    rdfs:isDefinedBy <>;
    .
